---
title: Higher Order Parital Derivatives
---

#### Second Order Partial Derivatives
>[!Info] Notation:
>$$(f_{x})_{x}=f_{xx}=\frac{∂}{∂x}\left( \frac{∂f}{∂x} \right)=\frac{∂^2f}{∂x^2}=\frac{∂^2z}{∂x^2}$$
>
>$$(f_{x})_{y}=f_{xy}=\frac{∂}{∂y}\left( \frac{∂f}{∂x} \right)=\frac{∂^2f}{∂y∂x}=\frac{∂^2z}{∂y∂x}$$
>
>$$(f_{y})_{x}=f_{yx}=\frac{∂}{∂x}\left( \frac{∂f}{∂y} \right)=\frac{∂^2f}{∂x∂y}=\frac{∂^2z}{∂x∂y}$$
>
>$$(f_{y})_{y}=f_{yy}=\frac{∂}{∂y}\left( \frac{∂f}{∂y} \right)=\frac{∂^2f}{∂y∂y}=\frac{∂^2z}{∂y∂y}$$

#### Higher-Order Derivatives
>[!Info] Notation
>Consider the function $f(x,y,z)$:
>
>$$f_{zyxy}=(((f_{z})_{y})_{x})_{y}=\frac{∂}{∂y}\left( \frac{∂}{∂x}\left( \frac{∂}{∂y}\left( \frac{∂f}{∂z} \right) \right) \right)=\frac{∂^4f}{∂y∂x∂y∂z}$$

#### Clairaut's Theorem
>[!abstract] Theorem
>If the function $f$ has continuous second-order partial derivatives, then:
>
>$$\frac{∂^2f}{∂x∂y}=\frac{∂^2f}{∂y∂x}$$

**Remark:** 
The theorem can be generalized to higher-order derivatives, and to functions of more than two variables.


