---
title: 4. Computation Rules and Standard Limits
---

#### Computation Rules
> [!abstract] Theorem (Sum Rule)
> Suppose
> 
> $$\lim_{ x \to \infty } f(x) = a$$ and $$\lim_{ x \to \infty } g(x) = b$$
> 
> then:
> 
> $$\lim_{ x \to \infty } f(x)+g(x) = \lim_{ x \to \infty } f(x) + \lim_{ x \to \infty } g(x) = a+b$$

> [!abstract] Theorem (Scale Rule)
> $$\lim_{ x \to \infty } cf(x) = c \lim_{ x \to \infty } f(x) = ca$$

> [!abstract] Theorem (Product Rule)
> $$\lim_{ x \to \infty } f(x)g(x) = (\lim_{ x \to \infty } f(x))(\lim_{ x \to \infty } g(x)) = ab$$

> [!abstract] Theorem (Quotient Rule)
> $$\lim_{ x \to \infty } \frac{f(x)}{g(x)} = \frac{\lim_{ x \to \infty } f(x)}{\lim_{ x \to \infty } g(x)} = \frac{a}{b}$$
> 
> if $b â‰  0$

> [!abstract] Theorem (Composition Rule)
> Suppose
> 
> $$\lim_{ x \to \infty } f(x) = a$$
> 
> and $h(x)$ does not have a jump at $x=a$, then:
> 
> $$\lim_{ x \to \infty } h(f(x)) = h(\lim_{ x \to \infty } f(x)) = h(a)$$

#### Standard Limits
> [!abstract] Theorem
> Suppose $r>0$ and $k$ is positive integer
> 
> $$\lim_{ x \to \pm\infty } c=c $$
> 
> $$\lim_{ x \to \infty } \frac{1}{x^r}=0$$
> 
> $$\lim_{ x \to -\infty } \frac{1}{x^k}=0$$
> 
> $$\lim_{ x \to \infty } e^{-rx} = 0$$
> 
> $$\lim_{ x \to -\infty } e^{rx} = 0$$

