---
title: 3. Differentiation Rules
---

>[!Standard Derivatives]
>
>$(x^r)' = rx^{r-1}$ for any real value $r$ (power of $x$)
>
>$(e^x)' = e^x$ (exponential function)
>
>$[e^{u(x)}]' = e^{u(x)} \cdot u'(x)$ (chain rule + exponential function)
>
>$(\ln{x})' = \frac{1}{x}$ (natural logarithm)
>
>$[\ln(u(x))]' = \frac{1}{u(x)} \cdot u'(x)$ (chain rule + natural logarithm)
>
>$(\sin(x))' = \cos(x)$ (sine function)
>
>$[\sin(u(x))]' = \cos(u(x)) \cdot u'(x)$ (chain rule + sine function)
>
>$(\cos(x))' = -\sin(x)$ (cosine function)
>
>$[\cos(u(x))]' = -\sin(u(x)) \cdot u'(x)$ (chain rule + cosine function)

>[!Computation Rules]
>$(cf(x))' = cf'(x)$ for any real value $c$
>
>$(f(x)+g(x))'=f'(x) + g'(x)$ (Sum Rule)
>
>$(f(x)g(x))' = f'(x)g(x) + f(x)g'(x)$ (Product Rule)
>
>$(\frac{f(x)}{g(x)})' = \frac{f'(x)g(x) - f(x)g'(x)}{(g(x))^2}$ (Quotient Rule)
>
>$f(g(x))' = f'(g(x))g'(x)$ (Chain Rule)




